Start converting to literate programming

Cpu.fst
@@ -1,25 +1,55 @@
-(* Top-level CPU model *)
+/// *******************
+/// Low-level CPU model
+/// *******************
 module Cpu
 
 open Memory
 open Value
 
+/// ============
+/// System state
+/// ============
+
+/// We start by defining the low-level state of the system.  We begin by defining memory
+/// types.
+///
+/// What does an address look like, and what does a word in memory look like?
 type address = FStar.UInt64.t
 type word = FStar.UInt64.t
 
+/// Furthermore what is the size of the memory?  Since an address is a UInt64, the
+/// memory should have at most :math:`2^{64}` cells.
 type memory_size = n:int{FStar.UInt.fits n FStar.UInt64.n}
 
+/// Next we describe the state of the caches.  We don't need to include the
+/// actual cache lines; for our purposes, an array of cache line assignments
+/// is enough.
 type cache_state (n:memory_size) =
        (list (a:address{FStar.UInt64.v a < n}))
 
-
+/// Finally, we can define the state of the overall system.  This type is
+/// parametrized by the sizes of the memory and register file, as described in
+/// §6.2.2 of the paper.
 type systemState (#n #r:memory_size)
      = { memory: (memory:memoryState{(FStar.List.length memory) = n});
     cache_lines: (list (a:address{FStar.UInt64.v a < n}));
              pc: (pc:word{FStar.UInt64.v pc < n});
       registers: (registers:memoryState{FStar.List.length registers = r})}
 
-(* Equivalence *)
+/// -----------
+/// Equivalence
+/// -----------
+///
+/// Next we define and analyze the notion of system equivalence, :math:`\stackrel{\mathrm{state}}{\equiv}`, as in §6.2.2 of the paper.
+///
+/// Two systems are in equivalent states if
+///   - their memory banks and register files have the same size,
+///   - their program counters point to the same address,
+///   - their cache line assignments are identical,
+///   - their memory banks and register files are equivalent, in the sense of :ref:`equiv_list <equiv_list>`
+///
+/// .. fst::
+///   :name: equiv_system
 let equiv_system (#m #q #n #r: memory_size) (lhs:systemState #m #q) (rhs:systemState #n #r)
     = (m = n)
        /\ (q = r)
@@ -29,12 +59,18 @@ let equiv_system (#m #q #n #r: memory_size) (lhs:systemState #m #q) (rhs:systemS
        /\ (equivalent_lists_have_equal_lengths lhs.memory rhs.memory;
           lhs.cache_lines = rhs.cache_lines)
 
+/// We then prove several properties of :math:`\stackrel{\mathrm{state}}{\equiv}`:
+///   - **Equality implies equivalence**: :math:`s_1 = s_2 \Rightarrow s_1 \stackrel{\mathrm{state}}{\equiv} s_2`
 let equal_systems_are_equivalent (#n #r:memory_size) (lhs:systemState #n #r) (rhs:systemState #n #r):
   Lemma (requires lhs = rhs) (ensures (equiv_system #n #r #n #r lhs rhs)) =
   equal_lists_are_equivalent _ lhs.registers rhs.registers;
   equal_lists_are_equivalent _ lhs.memory rhs.memory
 
-let system_equivalence_is_transitive (#m #q #n #r #o #s: memory_size) (lhs:systemState #m #q) (mid:systemState #n #r) (rhs:systemState #o #s):
+///   - **Transitivity**: :math:`s_1 \stackrel{\mathrm{state}}{\equiv} s_2 \wedge s_2 \stackrel{\mathrm{state}}{\equiv} s_3 \Rightarrow s_1 \stackrel{\mathrm{state}}{\equiv} s_3`
+let system_equivalence_is_transitive (#m #q #n #r #o #s: memory_size)
+                                     (lhs:systemState #m #q)
+                                     (mid:systemState #n #r)
+                                     (rhs:systemState #o #s):
     Lemma (requires (equiv_system lhs mid) /\ (equiv_system mid rhs))
           (ensures  equiv_system lhs rhs)
     = assert(lhs.pc = rhs.pc);
@@ -46,7 +82,10 @@ let system_equivalence_is_transitive (#m #q #n #r #o #s: memory_size) (lhs:syste
       assert(lhs.cache_lines = rhs.cache_lines)
 
 
-let system_equivalence_is_symmetric (#m #q #n #r: memory_size) (lhs: systemState #m #q) (rhs:systemState #n #r):
+///   - **Symmetry**: :math:`s_1 \stackrel{\mathrm{state}}{\equiv} s_2 \Leftrightarrow s_2 \stackrel{\mathrm{state}}{\equiv} s_1`
+let system_equivalence_is_symmetric (#m #q #n #r: memory_size)
+                                    (lhs: systemState #m #q)
+                                    (rhs:systemState #n #r):
     Lemma (requires equiv_system lhs rhs)
           (ensures  equiv_system rhs lhs)
     = assert(lhs.pc = rhs.pc);
@@ -57,14 +96,22 @@ let system_equivalence_is_symmetric (#m #q #n #r: memory_size) (lhs: systemState
       list_equivalence_is_symmetric _ lhs.registers rhs.registers;
       list_equivalence_is_symmetric _ lhs.memory          rhs.memory
 
-
-(*******************************************************************************
- * Redaction
- *
- * We introduce the concept of "redaction", which is to zero all of the data in
- * blinded values of the system.
- *******************************************************************************)
-
+/// ---------
+/// Redaction
+/// ---------
+///
+/// Equivalence is not always the easiest notion to work with, since the
+/// associated theorems often take the form of
+///
+/// .. math ::
+///
+///    \forall s_1, s_2. s_1 \stackrel{\mathrm{state}}{\equiv} s_2 \Rightarrow f(s_1) \stackrel{\mathrm{state}}{\equiv} f(s_2),
+///
+/// which we need to prove despite not knowing anything about :math:`s_1`
+/// or :math:`s_2` or their relationship to one another.
+///
+/// We introduce the concept of *redaction*, which is to zero all of the data in
+/// blinded values of the system.
 let redact_system (#n #r: memory_size) (s:systemState #n #r): systemState #n #r = {
     pc = (redaction_preserves_length _ s.memory 0uL;
           let redacted_memory = redact_list s.memory 0uL in
@@ -75,27 +122,57 @@ let redact_system (#n #r: memory_size) (s:systemState #n #r): systemState #n #r 
     memory    = redact_list s.memory 0uL
     }
 
-
+/// We then prove that systems are equivalent to their redaction:
 let systems_are_equivalent_to_their_redaction (#n #r: memory_size) (s:systemState #n #r):
     Lemma (ensures equiv_system s (redact_system s))
     = lists_are_equivalent_to_their_redaction  _ s.registers 0uL;
       lists_are_equivalent_to_their_redaction  _ s.memory 0uL
 
-let equivalent_systems_have_equal_redactions (#m #q #n #r: memory_size) (s1:systemState #m #q) (s2:systemState #n #r):
+/// and that the redactions of equivalent systems are equal:
+
+let equivalent_systems_have_equal_redactions (#m #q #n #r: memory_size)
+                                             (s1:systemState #m #q)
+                                             (s2:systemState #n #r):
     Lemma (requires (equiv_system s1 s2)) (ensures ((redact_system s1) == (redact_system s2)))
     = assert(m = n);
       equivalent_lists_have_equal_redactions _ s1.registers s2.registers 0uL;
       equivalent_lists_have_equal_redactions _ s1.memory s2.memory 0uL
 
+/// Together, these theorems let us more easily prove theorems of the form
+///
+/// .. math ::
+///
+///     \forall s_1, s_2: s_1 \stackrel{\mathrm{state}}{\equiv} s_2 \Rightarrow f(s_1) \stackrel{\mathrm{state}}{\equiv} f(s_2).
+///
+/// by instead proving that
+///
+/// .. math ::
+///
+///    \forall s: f(s) \stackrel{\mathrm{state}}{\equiv} f(\mathrm{redact}\; s)
+///
+/// which by ``systems_are_equivalent_to_their_redaction`` and ``equivalent_systems_have_equal_redactions`` yield
+///
+/// .. math ::
+///
+///    \forall s_1, s_2: s_1 \stackrel{\mathrm{state}}{\equiv} s_2 \Rightarrow  f(s_1) \stackrel{\mathrm{state}}{\equiv} f(\mathrm{redact}\; s_1) = f(\mathrm{redact}\; s_2) \stackrel{\mathrm{state}}{\equiv} f(s_2) .
+/// 
 
-(*******************************************************************************
- * System definition.
- *
- * We build our system from an execution unit (essentially, an ISA)
- * and a function that "steps" the processor state (essentially, the
- * microarchitecture, which for now just fetch-executes in a single step).
- *******************************************************************************)
+
+/// ===============
+/// Execution model
+/// ===============
+///
+/// The next step is to describe how the system actually executes.
+///
+/// We represent this using:
+///   - an execution unit (essentially, an ISA)
+///
+///     .. fst ::
 type execution_unit (#n #r:memory_size) = word -> systemState #n #r -> systemState #n #r
+
+///   - a function that "steps" the processor state, which in this case
+///     means to load an instruction from memory and execute it in a
+///     single cycle.
 
 val step (#n #r:memory_size)
     (exec:execution_unit #n #r)
@@ -108,28 +185,41 @@ let step exec pre_state =
         | Blinded _ -> { pre_state with pc = 0uL }
         | Clear inst -> exec inst pre_state
 
-(*******************************************************************************
- * Equivalence-based safety.
- *
- * We define safety in this case to be that the system is safe if executing on
- * equivalent (and so indistinguishable) states always results in equivalent
- * output states.
- *******************************************************************************)
-let equivalent_inputs_yield_equivalent_states (#n #r:memory_size) (exec:execution_unit #n #r) (pre1 pre2 : systemState #n #r) =
-    equiv_system pre1 pre2 ==> equiv_system (step exec pre1) (step exec pre2)
 
+/// ==================
+/// Safety definitions
+/// ==================
+///
+/// ------------------------
+/// Equivalence-based safety
+/// ------------------------
+///
+/// We define safety in this case to be that the system is safe if executing on
+/// equivalent (and so indistinguishable) states always results in equivalent
+/// output states.
+///
+/// We start by defining a test that checks whether this is the case for a
+/// particular set of equivalent initial states:
+
+let equivalent_inputs_yield_equivalent_states (#n #r:memory_size)
+                                              (exec:execution_unit #n #r)
+                                              (pre1:systemState #n #r)
+                                              (pre2:(systemState #n #r){equiv_system pre1 pre2}) =
+    equiv_system (step exec pre1) (step exec pre2)
+
+/// Then, we define safety by whether execution preserves state equivalence for
+/// *all* possible inputs.
 let is_safe (#n #r:memory_size) (exec:execution_unit #n #r) =
-    forall (pre1 pre2 : systemState). equivalent_inputs_yield_equivalent_states exec pre1 pre2
+    forall (pre1 pre2 : systemState). (equiv_system pre1 pre2) ==> equivalent_inputs_yield_equivalent_states exec pre1 pre2
 
 type safe_execution_unit (#n #r:memory_size) = exec:(execution_unit #n #r){is_safe exec}
 
-(*******************************************************************************
- * Redacting-equivalent execution units.
- *
- * We can show that a system constructed from an execution unit that produces
- * an equivalent output when operating on the same input but with the blinded
- * values zeroed is safe.
- *******************************************************************************)
+/// ----------------------
+/// Redaction-based safety
+/// ----------------------
+/// We can show that a system constructed from an execution unit that produces
+/// an equivalent output when operating on the same input but with the blinded
+/// values zeroed is safe.
 
  let is_redacting_equivalent_execution_unit (#n #r:memory_size) (exec:execution_unit #n #r)
    = forall(pre:systemState) (inst:word).  (equiv_system (exec inst pre) (exec inst (redact_system pre)))
@@ -137,14 +227,19 @@ type safe_execution_unit (#n #r:memory_size) = exec:(execution_unit #n #r){is_sa
 type redacting_equivalent_execution_unit (#n #r:memory_size)
    = exec:(execution_unit #n #r){is_redacting_equivalent_execution_unit exec}
 
-let is_redacting_equivalent_system_single_step_somewhere (#n #r:memory_size) (exec:execution_unit #n #r) (pre:systemState #n #r) =
+let is_redacting_equivalent_system_single_step_somewhere (#n #r:memory_size)
+                                                         (exec:execution_unit #n #r)
+                                                         (pre:systemState #n #r) =
     (equiv_system (step exec pre) (step exec (redact_system pre)))
 
-let is_redacting_equivalent_system_single_step_everywhere (#n #r:memory_size) (exec:execution_unit #n #r) =
+let is_redacting_equivalent_system_single_step_everywhere (#n #r:memory_size)
+                                                          (exec:execution_unit #n #r) =
     forall (pre:systemState). is_redacting_equivalent_system_single_step_somewhere exec pre
 
-let redacting_equivalent_execution_units_lead_to_redacting_equivalent_systems_somewhere (#n #r:memory_size)
-    (exec:redacting_equivalent_execution_unit #n #r) (pre:systemState #n #r):
+let redacting_equivalent_execution_units_lead_to_redacting_equivalent_systems_somewhere
+                                                          (#n #r:memory_size)
+                                                          (exec:redacting_equivalent_execution_unit #n #r)
+                                                          (pre:systemState #n #r):
     Lemma (ensures is_redacting_equivalent_system_single_step_somewhere exec pre) =
       let redaction = redact_system pre in
       systems_are_equivalent_to_their_redaction pre;
@@ -165,9 +260,13 @@ let redacting_equivalent_systems_give_equivalent_outputs_for_equivalent_inputs (
         assert( (step exec (redact_system pre_1)) == (step exec (redact_system pre_2)) );
         system_equivalence_is_symmetric (step exec pre_2) (step exec (redact_system pre_2));
         assert( equiv_system (step exec (redact_system pre_2)) (step exec pre_2) );
-        system_equivalence_is_transitive (step exec pre_1) (step exec (redact_system pre_1)) (step exec pre_2)
+        system_equivalence_is_transitive (step exec pre_1)
+                                         (step exec (redact_system pre_1))
+                                         (step exec pre_2)
 
-(* The main theorem about execution_units *)
+/// ------------
+/// Main theorem
+/// ------------
 let redacting_equivalent_execution_units_are_safe (#n #r:memory_size)
     (exec:redacting_equivalent_execution_unit #n #r):
     Lemma (ensures is_safe exec)
